Define repeats_trace

Itree.fst
@@ -688,11 +688,39 @@ let tio_call #a (o : cmds) (x : io_args o) #w (k : (r : io_res o) -> tio a (w r)
   ) ;
   call o x k
 
-// TODO of course
-assume val repeats_trace (t t' : trace) : Type0
+let rec consume_trace (t t' : trace) : option trace =
+  match t with
+  | [] -> Some []
+  | x :: t ->
+    begin match t' with
+    | [] -> None
+    | y :: t' ->
+      if x = y
+      then consume_trace t t'
+      else None
+    end
+
+let rec consume_trace_smaller (t t' : trace) :
+  Lemma (forall tt. consume_trace t t' == Some tt ==> t == [] \/ tt << t)
+= match t with
+  | [] -> ()
+  | x :: t ->
+    begin match t' with
+    | [] -> ()
+    | y :: t' ->
+      if x = y
+      then consume_trace_smaller t t'
+      else ()
+    end
+
+let rec repeats_trace (t t' : trace) : Type0 =
+  match consume_trace t t' with
+  | Some [] -> True
+  | Some tt -> consume_trace_smaller t t' ; repeats_trace tt t'
+  | None -> False
 
 let twp_repeat (w : twp unit) : twp unit =
-  fun post -> // Is it really the right spec?
+  fun post ->
     // Either the body doesn't terminate or it does and the trace is repeated
     w (fun tr v ->
       match v with
